src/ParamDup.v
@@ -1,0 +1,287 @@
+Require Import String List.
+Require Import Lib.CommonTactics Lib.Word Lib.Struct Lib.FMap Lib.Concat Lib.Indexer.
+Require Import Syntax Semantics SemFacts Specialize Duplicate Refinement ParametricSyntax.
+
+Lemma getMetaRegName_sinRegs:
+  forall {A} (strA: A -> string) Hgood1 Hgood2 {ls} (HnoDup: NoDup ls) sregs,
+    map getMetaRegName (regsToRep strA Hgood1 Hgood2 HnoDup sregs) =
+    map (fun sr => nameVal (regName sr)) sregs.
+Proof.
+  induction sregs; simpl; intros; auto.
+  destruct a; simpl; f_equal; auto.
+Qed.
+
+Lemma EquivList_cons:
+  forall {A} (a1 a2: A) l1 l2,
+    EquivList l1 l2 -> a1 = a2 -> EquivList (a1 :: l1) (a2 :: l2).
+Proof.
+  intros; inv H; subst; split;
+    try (apply SubList_cons; [left; auto|apply SubList_cons_right; auto]).
+Qed.
+
+Section SinModuleDup.
+
+  Lemma Specializable_weakening:
+    forall m1 m2,
+      Specializable m1 ->
+      SubList (namesOf (getRegInits m2)) (namesOf (getRegInits m1)) ->
+      SubList (namesOf (getRules m2)) (namesOf (getRules m1)) ->
+      SubList (getDefs m2) (getDefs m1) ->
+      SubList (getCalls m2) (getCalls m1) ->
+      Specializable m2.
+  Proof.
+    unfold Specializable, spDom; intros.
+    rewrite <-hasNoIndex_makeNoDup in *.
+    eapply hasNoIndex_SubList; eauto.
+    repeat (apply SubList_app_6; auto).
+  Qed.
+
+  Lemma renameListAttr_specializer_regs:
+    forall eregs regs rules dms i,
+      Specializable (Mod eregs rules dms) ->
+      SubList regs eregs ->
+      Renaming.renameListAttr (specializer (Mod eregs rules dms) i) regs =
+      Renaming.renameListAttr (spf i) regs.
+  Proof.
+    induction regs; simpl; intros; auto.
+    f_equal.
+    - unfold Renaming.renameAttr; f_equal.
+      apply specializer_dom; auto.
+      unfold spDom; apply makeNoDup_SubList_2.
+      apply in_or_app; left; simpl.
+      apply in_map; apply H0; left; auto.
+    - apply IHregs; auto.
+      apply SubList_cons_inv in H0; dest; auto.
+  Qed.
+
+  Lemma regsToRep_duplicate_regs_equiv:
+    forall rules dms n (l: list (SinReg nat)),
+      (forall sr, In sr l -> forall i j, regGen sr i = regGen sr j) ->
+      Specializable (Mod (map (fun sr => (nameVal (regName sr) :: regGen sr 0)%struct) l)
+                         rules dms) ->
+      EquivList
+        (concat
+           (map getListFromMetaReg
+                (regsToRep string_of_nat string_of_nat_into withIndex_index_eq
+                           (getNatListToN_NoDup n) l)))
+        (getRegInits
+           (duplicate
+              (Mod (map (fun sr => (nameVal (regName sr) :: regGen sr 0)%struct) l)
+                   rules dms) n)).
+  Proof.
+    intros; induction l; [simpl; induction n; [apply EquivList_nil|auto]|].
+    destruct a as [arg arn]; simpl.
+
+    assert (EquivList
+              ((getListFromRep string_of_nat arg (nameVal arn) (getNatListToN n))
+                 ++ (getRegInits
+                       (duplicate
+                          (Mod (map (fun sr => (nameVal (regName sr) :: regGen sr 0)%struct) l)
+                               rules dms) n)))
+              (getRegInits
+                 (duplicate
+                    (Mod
+                       (((nameVal arn :: arg 0)%struct)
+                          :: map (fun sr => (nameVal (regName sr) :: regGen sr 0)%struct) l)
+                       rules dms) n))).
+    { clear -H H0.
+      simpl in H0; generalize dependent H0.
+      generalize (map (fun sr => (nameVal (regName sr) :: regGen sr 0)%struct) l) as ml.
+      intros.
+      assert (Specializable (Mod ml rules dms)).
+      { eapply Specializable_weakening; eauto;
+        try (unfold getDefs, getCalls; simpl; apply SubList_refl).
+        simpl; apply SubList_cons_right, SubList_refl.
+      }
+      generalize dependent n; induction n.
+      
+      - simpl; apply EquivList_cons.
+        + rewrite renameListAttr_specializer_regs; [|auto|apply SubList_refl].
+          rewrite renameListAttr_specializer_regs; [|auto|apply SubList_cons_right, SubList_refl].
+          apply EquivList_refl.
+        + unfold Renaming.renameAttr; simpl; f_equal.
+          rewrite specializer_dom; auto.
+          apply makeNoDup_SubList_2; left; auto.
+      - generalize dependent IHn.
+        unfold duplicate at 3. fold (duplicate (Mod ml rules dms)).
+        generalize (duplicate (Mod ml rules dms) n) as nm1.
+        unfold duplicate at 2.
+        fold (duplicate (Mod ((nameVal arn :: arg 0)%struct :: ml) rules dms)).
+        generalize (duplicate (Mod ((nameVal arn :: arg 0)%struct :: ml) rules dms) n) as nm2.
+        simpl.
+        generalize (getListFromRep string_of_nat arg (nameVal arn) (getNatListToN n)) as rr1.
+        rewrite renameListAttr_specializer_regs; [|auto|apply SubList_refl].
+        rewrite renameListAttr_specializer_regs; [|auto|apply SubList_cons_right, SubList_refl].
+        generalize (Renaming.renameListAttr (spf (S n)) ml) as rr2.
+        intros.
+
+        apply EquivList_cons.
+        + inv IHn; split.
+          * repeat apply SubList_app_3.
+            { eapply SubList_app_2, SubList_app_4; eauto. }
+            { apply SubList_app_1, SubList_refl. }
+            { eapply SubList_app_2, SubList_app_5; eauto. }
+          * repeat apply SubList_app_3.
+            { apply SubList_app_2, SubList_app_1, SubList_refl. }
+            { apply SubList_app_comm; rewrite <-app_assoc.
+              apply SubList_app_2, SubList_app_comm; auto.
+            }
+        + unfold Renaming.renameAttr; rewrite specializer_dom; auto.
+          * f_equal; simpl. 
+            specialize (H {| regGen := arg; regName := arn |}).
+            apply H; left; auto.
+          * simpl; unfold spDom; apply makeNoDup_SubList_2.
+            apply in_or_app; left.
+            left; auto.
+    }
+
+    eapply EquivList_trans; [|apply H1]; clear H1.
+    apply EquivList_app; [apply EquivList_refl|].
+    apply IHl.
+    - clear -H; intros; apply H; right; auto.
+    - clear -H0.
+      eapply Specializable_weakening; eauto;
+        try (unfold getDefs, getCalls; simpl; apply SubList_refl).
+      simpl; apply SubList_cons_right, SubList_refl.
+  Qed.
+
+  Lemma renameRules_specializer_rules:
+    forall regs erules rules dms i,
+      Specializable (Mod regs erules dms) ->
+      SubList rules erules ->
+      Renaming.renameRules (specializer (Mod regs erules dms) i) rules =
+      Renaming.renameRules (spf i) rules.
+  Proof.
+    induction rules; simpl; intros; auto.
+    f_equal.
+    - destruct a as [an ar]; simpl; f_equal.
+      + apply specializer_dom; auto.
+        unfold spDom; apply makeNoDup_SubList_2.
+        apply in_or_app; right.
+        apply in_or_app; left; simpl.
+        apply SubList_cons_inv in H0; dest.
+        eapply in_map with (f:= @attrName _) in H0; eauto.
+      + admit.
+    - apply IHrules; auto.
+      apply SubList_cons_inv in H0; dest; auto.
+  Qed.
+
+  Lemma rulesToRep_duplicate_rules_equiv:
+    forall regs dms {genK} (getConst: nat -> ConstT genK) n (l: list SinRule),
+      Specializable
+        (Mod regs (map (fun sr => (nameVal (ruleName sr)
+                                           :: getActionFromSin (ruleGen sr))%struct) l) dms) ->
+      EquivList
+        (concat
+           (map getListFromMetaRule
+                (rulesToRep string_of_nat string_of_nat_into getConst withIndex_index_eq 
+                            (getNatListToN_NoDup n) 
+                            l)))
+        (getRules
+           (duplicate
+              (Mod regs (map (fun sr => (nameVal (ruleName sr)
+                                                 :: getActionFromSin (ruleGen sr))%struct) 
+                             l) dms) n)).
+  Proof.
+    intros; induction l; [simpl; induction n; [apply EquivList_nil|auto]|].
+    destruct a as [arg arn]; simpl.
+
+    assert (EquivList
+              ((repRule string_of_nat getConst (fun ty => convSinToGen true genK (arg ty))
+                        (nameVal arn) (getNatListToN n))
+                 ++ (getRules
+                       (duplicate
+                          (Mod regs
+                               (map (fun sr => (nameVal (ruleName sr)
+                                                        :: getActionFromSin (ruleGen sr))%struct)
+                                    l) dms) n)))
+              (getRules
+                 (duplicate
+                    (Mod regs
+                         (((nameVal arn :: getActionFromSin arg)%struct)
+                            :: (map
+                                  (fun sr : SinRule =>
+                                     (nameVal (ruleName sr)
+                                              :: getActionFromSin (ruleGen sr))%struct)
+                                  l)) dms) n))).
+    { clear -H.
+      simpl in H; generalize dependent H.
+      generalize (map (fun sr => (nameVal (ruleName sr) :: getActionFromSin (ruleGen sr))%struct)
+                      l) as ml.
+      intros.
+      assert (Specializable (Mod regs ml dms)).
+      { eapply Specializable_weakening; eauto; try (unfold getDefs; simpl; apply SubList_refl).
+        { simpl; apply SubList_cons_right, SubList_refl. }
+        { unfold getCalls; simpl.
+          rewrite <-app_assoc; apply SubList_app_2, SubList_refl.
+        }
+      }
+      generalize dependent n; induction n.
+      
+      - simpl; apply EquivList_cons.
+        + rewrite renameRules_specializer_rules; [|auto|apply SubList_refl].
+          rewrite renameRules_specializer_rules; [|auto|apply SubList_cons_right, SubList_refl].
+          apply EquivList_refl.
+        + f_equal.
+          * rewrite specializer_dom; auto.
+            apply makeNoDup_SubList_2.
+            apply in_or_app; right.
+            apply in_or_app; left.
+            simpl; auto.
+          * admit.
+      - admit.
+    }
+
+    eapply EquivList_trans; [|apply H0]; clear H0.
+    apply EquivList_app; [apply EquivList_refl|].
+    apply IHl.
+    - clear -H.
+      eapply Specializable_weakening; eauto; try (unfold getDefs; simpl; apply SubList_refl).
+      + simpl; apply SubList_cons_right, SubList_refl.
+      + unfold getCalls; simpl.
+        rewrite <-app_assoc; apply SubList_app_2, SubList_refl.
+  Qed.
+
+  Variable sm: SinModule nat.
+  Hypotheses
+    (* Hsp is provable generally, but fine to prove for each instantiation *)
+    (Hsp: Specializable (getModFromSin sm)) 
+    (HnoDupRegs: NoDup (map (fun sr => nameVal (regName sr)) (sinRegs sm)))
+    (HregInits: forall sr, In sr (sinRegs sm) -> forall i j, regGen sr i = regGen sr j).
+
+  Lemma sinModule_duplicate_1:
+    forall n, (modFromMeta (getMetaFromSinNat n sm) <<==
+                           duplicate (getModFromSin sm) (wordToNat (wones n))).
+  Proof.
+    intros; unfold MethsT; rewrite SemFacts.idElementwiseId.
+    apply traceRefines_same_module_structure.
+    - apply noDup_metaRegs.
+      simpl; rewrite getMetaRegName_sinRegs; auto.
+    - apply duplicate_regs_NoDup; auto.
+      p_equal HnoDupRegs; unfold getModFromSin; simpl.
+      clear; induction (sinRegs sm); simpl; auto.
+      f_equal; auto.
+    - apply regsToRep_duplicate_regs_equiv; auto.
+    - apply rulesToRep_duplicate_rules_equiv; auto.
+    - admit.
+  Qed.
+
+  Lemma sinModule_duplicate_2:
+    forall n, (duplicate (getModFromSin sm) (wordToNat (wones n)) <<==
+                         modFromMeta (getMetaFromSinNat n sm)).
+  Proof.
+    intros; unfold MethsT; rewrite SemFacts.idElementwiseId.
+    apply traceRefines_same_module_structure.
+    - apply duplicate_regs_NoDup; auto.
+      p_equal HnoDupRegs; unfold getModFromSin; simpl.
+      clear; induction (sinRegs sm); simpl; auto.
+      f_equal; auto.
+    - apply noDup_metaRegs.
+      simpl; rewrite getMetaRegName_sinRegs; auto.
+    - apply EquivList_comm, regsToRep_duplicate_regs_equiv; auto.
+    - apply EquivList_comm, rulesToRep_duplicate_rules_equiv; auto.
+    - admit.
+  Qed.
+
+End SinModuleDup.
+
